save

Source/DafnyCore/DafnyPrelude.bpl
@@ -662,7 +662,7 @@ function Set#Card<T>(Set T): int;
 axiom (forall<T> s: Set T :: { Set#Card(s) } 0 <= Set#Card(s));
 
 function Set#Empty<T>(): Set T;
-axiom (forall<T> o: T :: { Set#Empty()[o] } !Set#Empty()[o]);
+// axiom (forall<T> o: T :: { Set#Empty()[o] } !Set#Empty()[o]);
 axiom (forall<T> s: Set T :: { Set#Card(s) }
   (Set#Card(s) == 0 <==> s == Set#Empty()) &&
   (Set#Card(s) != 0 ==> (exists x: T :: s[x])));
@@ -951,226 +951,237 @@ axiom (forall<T> s: Seq T, i: int, v: T, x: T ::
     MultiSet#FromSeq(Seq#Update(s, i, v))[x] ==
       MultiSet#Union(MultiSet#Difference(MultiSet#FromSeq(s), MultiSet#Singleton(Seq#Index(s,i))), MultiSet#Singleton(v))[x] );
   // i.e. MS(Update(s, i, v)) == MS(s) - {{s[i]}} + {{v}}
-axiom (forall<T> s: Seq T, x: T :: { MultiSet#FromSeq(s)[x] }
-  (exists i : int :: { Seq#Index(s,i) } 0 <= i && i < Seq#Length(s) && x == Seq#Index(s,i)) <==> 0 < MultiSet#FromSeq(s)[x] );
+// axiom (forall<T> s: Seq T, x: T :: { MultiSet#FromSeq(s)[x] }
+//   (exists i : int :: { Seq#Index(s,i) } 0 <= i && i < Seq#Length(s) && x == Seq#Index(s,i)) <==> 0 < MultiSet#FromSeq(s)[x] );
 
 // ---------------------------------------------------------------
 // -- Axiomatization of sequences --------------------------------
 // ---------------------------------------------------------------
 
-type Seq T;
+type {:builtin "Seq"} Seq T;
 
-function Seq#Length<T>(Seq T): int;
-axiom (forall<T> s: Seq T :: { Seq#Length(s) } 0 <= Seq#Length(s));
+function {:builtin "seq.len"} Seq#Length<T>(Seq T): int;
+// axiom (forall<T> s: Seq T :: { Seq#Length(s) } 0 <= Seq#Length(s));
 
-function Seq#Empty<T>(): Seq T;
-axiom (forall<T> :: { Seq#Empty(): Seq T } Seq#Length(Seq#Empty(): Seq T) == 0);
-axiom (forall<T> s: Seq T :: { Seq#Length(s) }
-  (Seq#Length(s) == 0 ==> s == Seq#Empty())
+function {:builtin "seq.empty"} Seq#Empty<T>(): Seq T;
+// axiom (forall<T> :: { Seq#Empty(): Seq T } Seq#Length(Seq#Empty(): Seq T) == 0);
+// axiom (forall<T> s: Seq T :: { Seq#Length(s) }
+//   (Seq#Length(s) == 0 ==> s == Seq#Empty())
 // The following would be a nice fact to include, because it would enable verifying the
 // GenericPick.SeqPick* methods in Test/dafny0/SmallTests.dfy.  However, it substantially
 // slows down performance on some other tests, including running seemingly forever on
 // some.
 //  && (Seq#Length(s) != 0 ==> (exists x: T :: Seq#Contains(s, x)))
-  );
+  // );
 
 // The empty sequence $Is any type
 //axiom (forall<T> t: Ty :: {$Is(Seq#Empty(): Seq T, TSeq(t))} $Is(Seq#Empty(): Seq T, TSeq(t)));
 
-function Seq#Singleton<T>(T): Seq T;
-axiom (forall<T> t: T :: { Seq#Length(Seq#Singleton(t)) } Seq#Length(Seq#Singleton(t)) == 1);
+function {:builtin "seq.unit"} Seq#Singleton<T>(T): Seq T;
+// axiom (forall<T> t: T :: { Seq#Length(Seq#Singleton(t)) } Seq#Length(Seq#Singleton(t)) == 1);
 
-function Seq#Build<T>(s: Seq T, val: T): Seq T;
-function Seq#Build_inv0<T>(s: Seq T) : Seq T;
-function Seq#Build_inv1<T>(s: Seq T) : T;
-axiom (forall<T> s: Seq T, val: T ::
-  { Seq#Build(s, val) }
-  Seq#Build_inv0(Seq#Build(s, val)) == s &&
-  Seq#Build_inv1(Seq#Build(s, val)) == val);
+function {:inline} Seq#Build<T>(s: Seq T, val: T) : Seq T{
+  Seq#Append(s, Seq#Singleton(val))
+}
 
-axiom (forall<T> s: Seq T, v: T ::
-  { Seq#Build(s,v) }
-  Seq#Length(Seq#Build(s,v)) == 1 + Seq#Length(s));
-axiom (forall<T> s: Seq T, i: int, v: T :: { Seq#Index(Seq#Build(s,v), i) }
-  (i == Seq#Length(s) ==> Seq#Index(Seq#Build(s,v), i) == v) &&
-  (i != Seq#Length(s) ==> Seq#Index(Seq#Build(s,v), i) == Seq#Index(s, i)));
+// function Seq#Build_inv0<T>(s: Seq T) : Seq T;
+// function Seq#Build_inv1<T>(s: Seq T) : T;
+// axiom (forall<T> s: Seq T, val: T ::
+//   { Seq#Build(s, val) }
+//   Seq#Build_inv0(Seq#Build(s, val)) == s &&
+//   Seq#Build_inv1(Seq#Build(s, val)) == val);
+
+// axiom (forall<T> s: Seq T, v: T ::
+//   { Seq#Build(s,v) }
+//   Seq#Length(Seq#Build(s,v)) == 1 + Seq#Length(s));
+// axiom (forall<T> s: Seq T, i: int, v: T :: { Seq#Index(Seq#Build(s,v), i) }
+//   (i == Seq#Length(s) ==> Seq#Index(Seq#Build(s,v), i) == v) &&
+//   (i != Seq#Length(s) ==> Seq#Index(Seq#Build(s,v), i) == Seq#Index(s, i)));
 
 // Build preserves $Is
-axiom (forall s: Seq Box, bx: Box, t: Ty :: { $Is(Seq#Build(s,bx),TSeq(t)) }
-    $Is(s,TSeq(t)) && $IsBox(bx,t) ==> $Is(Seq#Build(s,bx),TSeq(t)));
+// axiom (forall s: Seq Box, bx: Box, t: Ty :: { $Is(Seq#Build(s,bx),TSeq(t)) }
+//     $Is(s,TSeq(t)) && $IsBox(bx,t) ==> $Is(Seq#Build(s,bx),TSeq(t)));
 
-function Seq#Create(ty: Ty, heap: Heap, len: int, init: HandleType): Seq Box;
-axiom (forall ty: Ty, heap: Heap, len: int, init: HandleType ::
-  { Seq#Length(Seq#Create(ty, heap, len, init): Seq Box) }
-  $IsGoodHeap(heap) && 0 <= len ==>
-  Seq#Length(Seq#Create(ty, heap, len, init): Seq Box) == len);
-axiom (forall ty: Ty, heap: Heap, len: int, init: HandleType, i: int ::
-  { Seq#Index(Seq#Create(ty, heap, len, init), i) }
-  $IsGoodHeap(heap) && 0 <= i && i < len ==>
-  Seq#Index(Seq#Create(ty, heap, len, init), i) == Apply1(TInt, TSeq(ty), heap, init, $Box(i)));
+// function Seq#Create(ty: Ty, heap: Heap, len: int, init: HandleType): Seq Box;
+// axiom (forall ty: Ty, heap: Heap, len: int, init: HandleType ::
+//   { Seq#Length(Seq#Create(ty, heap, len, init): Seq Box) }
+//   $IsGoodHeap(heap) && 0 <= len ==>
+//   Seq#Length(Seq#Create(ty, heap, len, init): Seq Box) == len);
+// axiom (forall ty: Ty, heap: Heap, len: int, init: HandleType, i: int ::
+//   { Seq#Index(Seq#Create(ty, heap, len, init), i) }
+//   $IsGoodHeap(heap) && 0 <= i && i < len ==>
+//   Seq#Index(Seq#Create(ty, heap, len, init), i) == Apply1(TInt, TSeq(ty), heap, init, $Box(i)));
 
-function Seq#Append<T>(Seq T, Seq T): Seq T;
-axiom (forall<T> s0: Seq T, s1: Seq T :: { Seq#Length(Seq#Append(s0,s1)) }
-  Seq#Length(Seq#Append(s0,s1)) == Seq#Length(s0) + Seq#Length(s1));
+function {:builtin "seq.++"} Seq#Append<T>(Seq T, Seq T): Seq T;
+// axiom (forall<T> s0: Seq T, s1: Seq T :: { Seq#Length(Seq#Append(s0,s1)) }
+//   Seq#Length(Seq#Append(s0,s1)) == Seq#Length(s0) + Seq#Length(s1));
 
-function Seq#Index<T>(Seq T, int): T;
-axiom (forall<T> t: T :: { Seq#Index(Seq#Singleton(t), 0) } Seq#Index(Seq#Singleton(t), 0) == t);
-axiom (forall<T> s0: Seq T, s1: Seq T, n: int :: { Seq#Index(Seq#Append(s0,s1), n) }
-  (n < Seq#Length(s0) ==> Seq#Index(Seq#Append(s0,s1), n) == Seq#Index(s0, n)) &&
-  (Seq#Length(s0) <= n ==> Seq#Index(Seq#Append(s0,s1), n) == Seq#Index(s1, n - Seq#Length(s0))));
+function {:builtin "seq.nth"} Seq#Index<T>(Seq T, int): T;
+// axiom (forall<T> t: T :: { Seq#Index(Seq#Singleton(t), 0) } Seq#Index(Seq#Singleton(t), 0) == t);
+// axiom (forall<T> s0: Seq T, s1: Seq T, n: int :: { Seq#Index(Seq#Append(s0,s1), n) }
+//   (n < Seq#Length(s0) ==> Seq#Index(Seq#Append(s0,s1), n) == Seq#Index(s0, n)) &&
+//   (Seq#Length(s0) <= n ==> Seq#Index(Seq#Append(s0,s1), n) == Seq#Index(s1, n - Seq#Length(s0))));
 
-function Seq#Update<T>(Seq T, int, T): Seq T;
-axiom (forall<T> s: Seq T, i: int, v: T :: { Seq#Length(Seq#Update(s,i,v)) }
-  0 <= i && i < Seq#Length(s) ==> Seq#Length(Seq#Update(s,i,v)) == Seq#Length(s));
-axiom (forall<T> s: Seq T, i: int, v: T, n: int :: { Seq#Index(Seq#Update(s,i,v),n) }
-  0 <= n && n < Seq#Length(s) ==>
-    (i == n ==> Seq#Index(Seq#Update(s,i,v),n) == v) &&
-    (i != n ==> Seq#Index(Seq#Update(s,i,v),n) == Seq#Index(s,n)));
+function {:builtin "seq.update"} Seq_Update_Sub<T>(s: Seq T, i: int , sub: Seq T): Seq T;
 
-function Seq#Contains<T>(Seq T, T): bool;
-axiom (forall<T> s: Seq T, x: T :: { Seq#Contains(s,x) }
-  Seq#Contains(s,x) <==>
-    (exists i: int :: { Seq#Index(s,i) } 0 <= i && i < Seq#Length(s) && Seq#Index(s,i) == x));
-axiom (forall<T> x: T ::
-  { Seq#Contains(Seq#Empty(), x) }
-  !Seq#Contains(Seq#Empty(), x));
+function {:inline} Seq#Update<T>(s: Seq T, i: int, val: T): Seq T{
+  Seq_Update_Sub(s, i, Seq#Singleton(val))
+}
+// axiom (forall<T> s: Seq T, i: int, v: T :: { Seq#Length(Seq#Update(s,i,v)) }
+//   0 <= i && i < Seq#Length(s) ==> Seq#Length(Seq#Update(s,i,v)) == Seq#Length(s));
+// axiom (forall<T> s: Seq T, i: int, v: T, n: int :: { Seq#Index(Seq#Update(s,i,v),n) }
+//   0 <= n && n < Seq#Length(s) ==>
+//     (i == n ==> Seq#Index(Seq#Update(s,i,v),n) == v) &&
+//     (i != n ==> Seq#Index(Seq#Update(s,i,v),n) == Seq#Index(s,n)));
 
-axiom (forall<T> s0: Seq T, s1: Seq T, x: T ::
-  { Seq#Contains(Seq#Append(s0, s1), x) }
-  Seq#Contains(Seq#Append(s0, s1), x) <==>
-    Seq#Contains(s0, x) || Seq#Contains(s1, x));
+function {:builtin "seq.contains"} Seq_Contains_Sub<T>(Seq T, Seq T): bool;
 
-axiom (forall<T> s: Seq T, v: T, x: T ::  // needed to prove things like '4 in [2,3,4]', see method TestSequences0 in SmallTests.dfy
-  { Seq#Contains(Seq#Build(s, v), x) }
-    Seq#Contains(Seq#Build(s, v), x) <==> (v == x || Seq#Contains(s, x)));
+function {:inline} Seq#Contains<T>(s: Seq T, x:T): bool{
+  Seq_Contains_Sub(s, Seq#Singleton(x))
+}
+// axiom (forall<T> s: Seq T, x: T :: { Seq#Contains(s,x) }
+//   Seq#Contains(s,x) <==>
+//     (exists i: int :: { Seq#Index(s,i) } 0 <= i && i < Seq#Length(s) && Seq#Index(s,i) == x));
+// axiom (forall<T> x: T ::
+//   { Seq#Contains(Seq#Empty(), x) }
+//   !Seq#Contains(Seq#Empty(), x));
 
-axiom (forall<T> s: Seq T, n: int, x: T ::
-  { Seq#Contains(Seq#Take(s, n), x) }
-  Seq#Contains(Seq#Take(s, n), x) <==>
-    (exists i: int :: { Seq#Index(s, i) }
-      0 <= i && i < n && i < Seq#Length(s) && Seq#Index(s, i) == x));
-axiom (forall<T> s: Seq T, n: int, x: T ::
-  { Seq#Contains(Seq#Drop(s, n), x) }
-  Seq#Contains(Seq#Drop(s, n), x) <==>
-    (exists i: int :: { Seq#Index(s, i) }
-      0 <= n && n <= i && i < Seq#Length(s) && Seq#Index(s, i) == x));
+// axiom (forall<T> s0: Seq T, s1: Seq T, x: T ::
+//   { Seq#Contains(Seq#Append(s0, s1), x) }
+//   Seq#Contains(Seq#Append(s0, s1), x) <==>
+//     Seq#Contains(s0, x) || Seq#Contains(s1, x));
 
-function Seq#Equal<T>(Seq T, Seq T): bool;
-axiom (forall<T> s0: Seq T, s1: Seq T :: { Seq#Equal(s0,s1) }
-  Seq#Equal(s0,s1) <==>
-    Seq#Length(s0) == Seq#Length(s1) &&
-    (forall j: int :: { Seq#Index(s0,j) } { Seq#Index(s1,j) }
-        0 <= j && j < Seq#Length(s0) ==> Seq#Index(s0,j) == Seq#Index(s1,j)));
-axiom (forall<T> a: Seq T, b: Seq T :: { Seq#Equal(a,b) }  // extensionality axiom for sequences
-  Seq#Equal(a,b) ==> a == b);
+// axiom (forall<T> s: Seq T, v: T, x: T ::  // needed to prove things like '4 in [2,3,4]', see method TestSequences0 in SmallTests.dfy
+//   { Seq#Contains(Seq#Build(s, v), x) }
+//     Seq#Contains(Seq#Build(s, v), x) <==> (v == x || Seq#Contains(s, x)));
 
-function Seq#SameUntil<T>(Seq T, Seq T, int): bool;
-axiom (forall<T> s0: Seq T, s1: Seq T, n: int :: { Seq#SameUntil(s0,s1,n) }
-  Seq#SameUntil(s0,s1,n) <==>
-    (forall j: int :: { Seq#Index(s0,j) } { Seq#Index(s1,j) }
-        0 <= j && j < n ==> Seq#Index(s0,j) == Seq#Index(s1,j)));
+// axiom (forall<T> s: Seq T, n: int, x: T ::
+//   { Seq#Contains(Seq#Take(s, n), x) }
+//   Seq#Contains(Seq#Take(s, n), x) <==>
+//     (exists i: int :: { Seq#Index(s, i) }
+//       0 <= i && i < n && i < Seq#Length(s) && Seq#Index(s, i) == x));
+// axiom (forall<T> s: Seq T, n: int, x: T ::
+//   { Seq#Contains(Seq#Drop(s, n), x) }
+//   Seq#Contains(Seq#Drop(s, n), x) <==>
+//     (exists i: int :: { Seq#Index(s, i) }
+//       0 <= n && n <= i && i < Seq#Length(s) && Seq#Index(s, i) == x));
+// ----------------------------
+// function Seq#Equal<T>(Seq T, Seq T): bool;
+// axiom (forall<T> s0: Seq T, s1: Seq T :: { Seq#Equal(s0,s1) }
+//   Seq#Equal(s0,s1) <==>
+//     Seq#Length(s0) == Seq#Length(s1) &&
+//     (forall j: int :: { Seq#Index(s0,j) } { Seq#Index(s1,j) }
+//         0 <= j && j < Seq#Length(s0) ==> Seq#Index(s0,j) == Seq#Index(s1,j)));
+// axiom (forall<T> a: Seq T, b: Seq T :: { Seq#Equal(a,b) }  // extensionality axiom for sequences
+//   Seq#Equal(a,b) ==> a == b);
 
-function Seq#Take<T>(s: Seq T, howMany: int): Seq T;
-axiom (forall<T> s: Seq T, n: int :: { Seq#Length(Seq#Take(s,n)) }
-  0 <= n && n <= Seq#Length(s) ==> Seq#Length(Seq#Take(s,n)) == n);
-axiom (forall<T> s: Seq T, n: int, j: int ::
-  {:weight 25}
-  { Seq#Index(Seq#Take(s,n), j) }
-  { Seq#Index(s, j), Seq#Take(s,n) }
-  0 <= j && j < n && j < Seq#Length(s) ==>
-    Seq#Index(Seq#Take(s,n), j) == Seq#Index(s, j));
+// function Seq#SameUntil<T>(Seq T, Seq T, int): bool;
+// axiom (forall<T> s0: Seq T, s1: Seq T, n: int :: { Seq#SameUntil(s0,s1,n) }
+//   Seq#SameUntil(s0,s1,n) <==>
+//     (forall j: int :: { Seq#Index(s0,j) } { Seq#Index(s1,j) }
+//         0 <= j && j < n ==> Seq#Index(s0,j) == Seq#Index(s1,j)));
 
-function Seq#Drop<T>(s: Seq T, howMany: int): Seq T;
-axiom (forall<T> s: Seq T, n: int :: { Seq#Length(Seq#Drop(s,n)) }
-  0 <= n && n <= Seq#Length(s) ==> Seq#Length(Seq#Drop(s,n)) == Seq#Length(s) - n);
-axiom (forall<T> s: Seq T, n: int, j: int ::
-  {:weight 25}
-  { Seq#Index(Seq#Drop(s,n), j) }
-  0 <= n && 0 <= j && j < Seq#Length(s)-n ==>
-    Seq#Index(Seq#Drop(s,n), j) == Seq#Index(s, j+n));
-axiom (forall<T> s: Seq T, n: int, k: int ::
-  {:weight 25}
-  { Seq#Index(s, k), Seq#Drop(s,n) }
-  0 <= n && n <= k && k < Seq#Length(s) ==>
-    Seq#Index(Seq#Drop(s,n), k-n) == Seq#Index(s, k));
+// function Seq#Take<T>(s: Seq T, howMany: int): Seq T;
+// axiom (forall<T> s: Seq T, n: int :: { Seq#Length(Seq#Take(s,n)) }
+//   0 <= n && n <= Seq#Length(s) ==> Seq#Length(Seq#Take(s,n)) == n);
+// axiom (forall<T> s: Seq T, n: int, j: int ::
+//   {:weight 25}
+//   { Seq#Index(Seq#Take(s,n), j) }
+//   { Seq#Index(s, j), Seq#Take(s,n) }
+//   0 <= j && j < n && j < Seq#Length(s) ==>
+//     Seq#Index(Seq#Take(s,n), j) == Seq#Index(s, j));
 
-axiom (forall<T> s, t: Seq T, n: int ::
-  { Seq#Take(Seq#Append(s, t), n) }
-  { Seq#Drop(Seq#Append(s, t), n) }
-  n == Seq#Length(s)
-  ==>
-  Seq#Take(Seq#Append(s, t), n) == s &&
-  Seq#Drop(Seq#Append(s, t), n) == t);
+// function Seq#Drop<T>(s: Seq T, howMany: int): Seq T;
+// axiom (forall<T> s: Seq T, n: int :: { Seq#Length(Seq#Drop(s,n)) }
+//   0 <= n && n <= Seq#Length(s) ==> Seq#Length(Seq#Drop(s,n)) == Seq#Length(s) - n);
+// axiom (forall<T> s: Seq T, n: int, j: int ::
+//   {:weight 25}
+//   { Seq#Index(Seq#Drop(s,n), j) }
+//   0 <= n && 0 <= j && j < Seq#Length(s)-n ==>
+//     Seq#Index(Seq#Drop(s,n), j) == Seq#Index(s, j+n));
+// axiom (forall<T> s: Seq T, n: int, k: int ::
+//   {:weight 25}
+//   { Seq#Index(s, k), Seq#Drop(s,n) }
+//   0 <= n && n <= k && k < Seq#Length(s) ==>
+//     Seq#Index(Seq#Drop(s,n), k-n) == Seq#Index(s, k));
 
-function Seq#FromArray(h: Heap, a: ref): Seq Box;
-axiom (forall h: Heap, a: ref ::
-  { Seq#Length(Seq#FromArray(h,a)) }
-  Seq#Length(Seq#FromArray(h, a)) == _System.array.Length(a));
-axiom (forall h: Heap, a: ref ::
-  { Seq#FromArray(h, a) }
-  (forall i: int ::
-    // it's important to include both triggers, so that assertions about the
-    // the relation between the array and the sequence can be proved in either
-    // direction
-    { read(h, a, IndexField(i)) }
-    { Seq#Index(Seq#FromArray(h, a): Seq Box, i) }
-    0 <= i &&
-    i < Seq#Length(Seq#FromArray(h, a))  // this will trigger the previous axiom to get a connection with _System.array.Length(a)
-    ==>
-    Seq#Index(Seq#FromArray(h, a), i) == read(h, a, IndexField(i))));
-axiom (forall h0, h1: Heap, a: ref ::
-  { Seq#FromArray(h1, a), $HeapSucc(h0, h1) }
-  $IsGoodHeap(h0) && $IsGoodHeap(h1) && $HeapSucc(h0, h1) && h0[a] == h1[a]
-  ==>
-  Seq#FromArray(h0, a) == Seq#FromArray(h1, a));
-axiom (forall h: Heap, i: int, v: Box, a: ref ::
-  { Seq#FromArray(update(h, a, IndexField(i), v), a) }
-    0 <= i && i < _System.array.Length(a) ==> Seq#FromArray(update(h, a, IndexField(i), v), a) == Seq#Update(Seq#FromArray(h, a), i, v) );
+// axiom (forall<T> s, t: Seq T, n: int ::
+//   { Seq#Take(Seq#Append(s, t), n) }
+//   { Seq#Drop(Seq#Append(s, t), n) }
+//   n == Seq#Length(s)
+//   ==>
+//   Seq#Take(Seq#Append(s, t), n) == s &&
+//   Seq#Drop(Seq#Append(s, t), n) == t);
 
-// Commutability of Take and Drop with Update.
-axiom (forall<T> s: Seq T, i: int, v: T, n: int ::
-        { Seq#Take(Seq#Update(s, i, v), n) }
-        0 <= i && i < n && n <= Seq#Length(s) ==> Seq#Take(Seq#Update(s, i, v), n) == Seq#Update(Seq#Take(s, n), i, v) );
-axiom (forall<T> s: Seq T, i: int, v: T, n: int ::
-        { Seq#Take(Seq#Update(s, i, v), n) }
-        n <= i && i < Seq#Length(s) ==> Seq#Take(Seq#Update(s, i, v), n) == Seq#Take(s, n));
-axiom (forall<T> s: Seq T, i: int, v: T, n: int ::
-        { Seq#Drop(Seq#Update(s, i, v), n) }
-        0 <= n && n <= i && i < Seq#Length(s) ==> Seq#Drop(Seq#Update(s, i, v), n) == Seq#Update(Seq#Drop(s, n), i-n, v) );
-axiom (forall<T> s: Seq T, i: int, v: T, n: int ::
-        { Seq#Drop(Seq#Update(s, i, v), n) }
-        0 <= i && i < n && n <= Seq#Length(s) ==> Seq#Drop(Seq#Update(s, i, v), n) == Seq#Drop(s, n));
-// Extension axiom, triggers only on Takes from arrays.
-axiom (forall h: Heap, a: ref, n0, n1: int ::
-        { Seq#Take(Seq#FromArray(h, a), n0), Seq#Take(Seq#FromArray(h, a), n1) }
-        n0 + 1 == n1 && 0 <= n0 && n1 <= _System.array.Length(a) ==> Seq#Take(Seq#FromArray(h, a), n1) == Seq#Build(Seq#Take(Seq#FromArray(h, a), n0), read(h, a, IndexField(n0): Field Box)) );
-// drop commutes with build.
-axiom (forall<T> s: Seq T, v: T, n: int ::
-        { Seq#Drop(Seq#Build(s, v), n) }
-        0 <= n && n <= Seq#Length(s) ==> Seq#Drop(Seq#Build(s, v), n) == Seq#Build(Seq#Drop(s, n), v) );
+// function Seq#FromArray(h: Heap, a: ref): Seq Box;
+// axiom (forall h: Heap, a: ref ::
+//   { Seq#Length(Seq#FromArray(h,a)) }
+//   Seq#Length(Seq#FromArray(h, a)) == _System.array.Length(a));
+// axiom (forall h: Heap, a: ref ::
+//   { Seq#FromArray(h, a) }
+//   (forall i: int ::
+//     // it's important to include both triggers, so that assertions about the
+//     // the relation between the array and the sequence can be proved in either
+//     // direction
+//     { read(h, a, IndexField(i)) }
+//     { Seq#Index(Seq#FromArray(h, a): Seq Box, i) }
+//     0 <= i &&
+//     i < Seq#Length(Seq#FromArray(h, a))  // this will trigger the previous axiom to get a connection with _System.array.Length(a)
+//     ==>
+//     Seq#Index(Seq#FromArray(h, a), i) == read(h, a, IndexField(i))));
+// axiom (forall h0, h1: Heap, a: ref ::
+//   { Seq#FromArray(h1, a), $HeapSucc(h0, h1) }
+//   $IsGoodHeap(h0) && $IsGoodHeap(h1) && $HeapSucc(h0, h1) && h0[a] == h1[a]
+//   ==>
+//   Seq#FromArray(h0, a) == Seq#FromArray(h1, a));
+// axiom (forall h: Heap, i: int, v: Box, a: ref ::
+//   { Seq#FromArray(update(h, a, IndexField(i), v), a) }
+//     0 <= i && i < _System.array.Length(a) ==> Seq#FromArray(update(h, a, IndexField(i), v), a) == Seq#Update(Seq#FromArray(h, a), i, v) );
 
-function Seq#Rank<T>(Seq T): int;
-axiom (forall s: Seq Box, i: int ::
-        { DtRank($Unbox(Seq#Index(s, i)): DatatypeType) }
-        0 <= i && i < Seq#Length(s) ==> DtRank($Unbox(Seq#Index(s, i)): DatatypeType) < Seq#Rank(s) );
-axiom (forall<T> s: Seq T, i: int ::
-        { Seq#Rank(Seq#Drop(s, i)) }
-        0 < i && i <= Seq#Length(s) ==> Seq#Rank(Seq#Drop(s, i)) < Seq#Rank(s) );
-axiom (forall<T> s: Seq T, i: int ::
-        { Seq#Rank(Seq#Take(s, i)) }
-        0 <= i && i < Seq#Length(s) ==> Seq#Rank(Seq#Take(s, i)) < Seq#Rank(s) );
-axiom (forall<T> s: Seq T, i: int, j: int ::
-        { Seq#Rank(Seq#Append(Seq#Take(s, i), Seq#Drop(s, j))) }
-        0 <= i && i < j && j <= Seq#Length(s) ==> Seq#Rank(Seq#Append(Seq#Take(s, i), Seq#Drop(s, j))) < Seq#Rank(s) );
+// // Commutability of Take and Drop with Update.
+// axiom (forall<T> s: Seq T, i: int, v: T, n: int ::
+//         { Seq#Take(Seq#Update(s, i, v), n) }
+//         0 <= i && i < n && n <= Seq#Length(s) ==> Seq#Take(Seq#Update(s, i, v), n) == Seq#Update(Seq#Take(s, n), i, v) );
+// axiom (forall<T> s: Seq T, i: int, v: T, n: int ::
+//         { Seq#Take(Seq#Update(s, i, v), n) }
+//         n <= i && i < Seq#Length(s) ==> Seq#Take(Seq#Update(s, i, v), n) == Seq#Take(s, n));
+// axiom (forall<T> s: Seq T, i: int, v: T, n: int ::
+//         { Seq#Drop(Seq#Update(s, i, v), n) }
+//         0 <= n && n <= i && i < Seq#Length(s) ==> Seq#Drop(Seq#Update(s, i, v), n) == Seq#Update(Seq#Drop(s, n), i-n, v) );
+// axiom (forall<T> s: Seq T, i: int, v: T, n: int ::
+//         { Seq#Drop(Seq#Update(s, i, v), n) }
+//         0 <= i && i < n && n <= Seq#Length(s) ==> Seq#Drop(Seq#Update(s, i, v), n) == Seq#Drop(s, n));
+// // Extension axiom, triggers only on Takes from arrays.
+// axiom (forall h: Heap, a: ref, n0, n1: int ::
+//         { Seq#Take(Seq#FromArray(h, a), n0), Seq#Take(Seq#FromArray(h, a), n1) }
+//         n0 + 1 == n1 && 0 <= n0 && n1 <= _System.array.Length(a) ==> Seq#Take(Seq#FromArray(h, a), n1) == Seq#Build(Seq#Take(Seq#FromArray(h, a), n0), read(h, a, IndexField(n0): Field Box)) );
+// // drop commutes with build.
+// axiom (forall<T> s: Seq T, v: T, n: int ::
+//         { Seq#Drop(Seq#Build(s, v), n) }
+//         0 <= n && n <= Seq#Length(s) ==> Seq#Drop(Seq#Build(s, v), n) == Seq#Build(Seq#Drop(s, n), v) );
 
-// Additional axioms about common things
-axiom (forall<T> s: Seq T, n: int :: { Seq#Drop(s, n) }
-        n == 0 ==> Seq#Drop(s, n) == s);
-axiom (forall<T> s: Seq T, n: int :: { Seq#Take(s, n) }
-        n == 0 ==> Seq#Take(s, n) == Seq#Empty());
-axiom (forall<T> s: Seq T, m, n: int :: { Seq#Drop(Seq#Drop(s, m), n) }
-        0 <= m && 0 <= n && m+n <= Seq#Length(s) ==>
-        Seq#Drop(Seq#Drop(s, m), n) == Seq#Drop(s, m+n));
+// function Seq#Rank<T>(Seq T): int;
+// axiom (forall s: Seq Box, i: int ::
+//         { DtRank($Unbox(Seq#Index(s, i)): DatatypeType) }
+//         0 <= i && i < Seq#Length(s) ==> DtRank($Unbox(Seq#Index(s, i)): DatatypeType) < Seq#Rank(s) );
+// axiom (forall<T> s: Seq T, i: int ::
+//         { Seq#Rank(Seq#Drop(s, i)) }
+//         0 < i && i <= Seq#Length(s) ==> Seq#Rank(Seq#Drop(s, i)) < Seq#Rank(s) );
+// axiom (forall<T> s: Seq T, i: int ::
+//         { Seq#Rank(Seq#Take(s, i)) }
+//         0 <= i && i < Seq#Length(s) ==> Seq#Rank(Seq#Take(s, i)) < Seq#Rank(s) );
+// axiom (forall<T> s: Seq T, i: int, j: int ::
+//         { Seq#Rank(Seq#Append(Seq#Take(s, i), Seq#Drop(s, j))) }
+//         0 <= i && i < j && j <= Seq#Length(s) ==> Seq#Rank(Seq#Append(Seq#Take(s, i), Seq#Drop(s, j))) < Seq#Rank(s) );
+
+// // Additional axioms about common things
+// axiom (forall<T> s: Seq T, n: int :: { Seq#Drop(s, n) }
+//         n == 0 ==> Seq#Drop(s, n) == s);
+// axiom (forall<T> s: Seq T, n: int :: { Seq#Take(s, n) }
+//         n == 0 ==> Seq#Take(s, n) == Seq#Empty());
+// axiom (forall<T> s: Seq T, m, n: int :: { Seq#Drop(Seq#Drop(s, m), n) }
+//         0 <= m && 0 <= n && m+n <= Seq#Length(s) ==>
+//         Seq#Drop(Seq#Drop(s, m), n) == Seq#Drop(s, m+n));
 
 // ---------------------------------------------------------------
 // -- Axiomatization of Maps -------------------------------------
